started refinment to HOL-tail

Cook_Levin/IMP-_To_SAS+/IMP-_To_IMP--/Binary_Arithmetic_Nat.thy
@@ -8,6 +8,12 @@ fun nth_bit_of_num_nat :: "nat \<Rightarrow> nat \<Rightarrow> nat" where
                             if n = 0 then (if hd_nat x = 0 then 0 else 1) else
                             nth_bit_of_num_nat (tl_nat x) (n-1)) "
 
+definition nth_bit_of_num_tail ::"nat \<Rightarrow> nat \<Rightarrow> nat" where 
+"nth_bit_of_num_tail x n =  nth_bit_of_num_nat x n"
+
+lemma subtail_nth_bit_of_num :"nth_bit_of_num_tail x n =  nth_bit_of_num_nat x n"
+  using nth_bit_of_num_tail_def by simp
+
 lemma sub_nth_bit_of_num: "nth_bit_of_num_nat (num_encode x) n = bit_encode (nth_bit_of_num x n)"
      apply (subst nth_bit_of_num_nat.simps)
   apply (induct x n rule:nth_bit_of_num.induct)
@@ -37,6 +43,47 @@ fun nth_carry_nat :: "nat \<Rightarrow> nat \<Rightarrow> nat \<Rightarrow> nat"
   \<or> ((nth_bit_nat a n = 1 \<or> nth_bit_nat b n = 1) \<and> nth_carry_nat (n-1) a b = 1) 
   then 1 else 0) )"
 
+fun nth_carry_acc :: "nat \<Rightarrow> nat \<Rightarrow> nat \<Rightarrow> nat \<Rightarrow> nat \<Rightarrow>nat" where 
+"nth_carry_acc acc diff n a b = (if diff = 0 then acc else 
+if diff>n then (if (nth_bit_tail a 0 = 1 \<and> nth_bit_tail b 0 = 1) then nth_carry_acc 1 n n a b
+   else  nth_carry_acc 0 n n a b )
+else (if (nth_bit_tail a (n-diff+1) = 1 \<and> nth_bit_tail b (n-diff+1) = 1) 
+  \<or> ((nth_bit_tail a (n-diff+1) = 1 \<or> nth_bit_tail b (n-diff+1) = 1) \<and> (acc = 1)) 
+  then nth_carry_acc 1 (diff-1) n a b else nth_carry_acc 0 (diff-1) n a b))"
+
+lemma nth_carry_step:"diff < n \<Longrightarrow> nth_carry_acc (nth_carry_nat (n- Suc diff) a b ) (Suc diff) n a b 
+=  nth_carry_acc (nth_carry_nat (n-diff) a b) diff n a b "
+  apply (subst (1) nth_carry_acc.simps )
+  apply (auto simp add: Suc_diff_Suc subtail_nth_bit
+            simp del: nth_carry_acc.simps nth_bit_nat.simps nth_carry_nat.simps simp flip: One_nat_def) 
+  apply (auto  simp add: subtail_nth_bit)
+  done
+
+
+lemma nth_carry_induct:"diff \<le>n \<Longrightarrow> nth_carry_acc (nth_carry_nat (n-diff) a b) diff n a b
+= nth_carry_nat n a b"
+  apply (induct diff)
+  apply simp
+   apply (auto simp add: nth_carry_step simp del:nth_carry_acc.simps nth_carry_nat.simps )
+  done
+
+lemma nth_carry_base:"nth_carry_nat 0 a b = (if (nth_bit_nat a 0 = 1 \<and> nth_bit_nat b 0 = 1) 
+            then 1 else 0)" 
+  apply auto
+  done
+
+definition nth_carry_tail :: "nat \<Rightarrow> nat \<Rightarrow> nat \<Rightarrow> nat" where 
+"nth_carry_tail n a b = nth_carry_acc 0 (Suc n) n a b"
+
+lemma subtail_nth_carry:
+"nth_carry_tail n a b
+= nth_carry_nat n a b"
+  apply (auto simp only: nth_carry_tail_def)
+  apply (subst nth_carry_acc.simps)
+  using nth_carry_induct[of n n a b] nth_carry_base subtail_nth_bit
+   apply (auto simp add:  simp del:nth_carry_acc.simps nth_carry_nat.simps nth_bit_nat.simps )
+  done
+
 lemma sub_nth_carry: "nth_carry_nat n a b = bit_encode (nth_carry n a b)"
   apply (induct n)
   apply (auto simp add: sub_nth_bit)
@@ -45,17 +92,57 @@ lemma sub_nth_carry: "nth_carry_nat n a b = bit_encode (nth_carry n a b)"
 
 
 fun nth_carry_sub_nat :: "nat \<Rightarrow> nat \<Rightarrow> nat \<Rightarrow> nat" where
-"nth_carry_sub_nat n a b = (if n =0 then (if (nth_bit_nat a 0 = 0 \<and> nth_bit_nat b 0 = 1) then 1 else 0)
-else (if (nth_bit_nat a n = 0 \<and> ( nth_bit_nat b n = 1 \<or> nth_carry_sub_nat (n-1) a b = 1))
-    \<or> (nth_bit_nat a n = 1 \<and> (nth_bit_nat b n) = 1 \<and> nth_carry_sub_nat (n-1) a b = 1) then 1
-  else 0))"
+"nth_carry_sub_nat n a b = (if n =0 
+    then (if (nth_bit_nat a 0 = 0 \<and> nth_bit_nat b 0 = 1) 
+            then 1 else 0)
+    else (if (nth_bit_nat a n = 0 \<and> ( nth_bit_nat b n = 1 \<or> nth_carry_sub_nat (n-1) a b = 1))
+                \<or> (nth_bit_nat a n = 1 \<and> (nth_bit_nat b n) = 1 \<and> nth_carry_sub_nat (n-1) a b = 1)
+           then 1
+            else 0))"
 
-lemma sub_nth_carry_sub :"nth_carry_sub_nat n a b = bit_encode (nth_carry_sub n a b)"
- apply (induct n)
-  apply (auto simp add: sub_nth_bit)
+fun nth_carry_sub_acc :: "nat \<Rightarrow> nat \<Rightarrow> nat \<Rightarrow> nat \<Rightarrow> nat \<Rightarrow> nat" where 
+"nth_carry_sub_acc acc diff n a b = (if diff = 0 then acc else 
+(if diff > n 
+    then (if (nth_bit_tail a 0 = 0 \<and> nth_bit_tail b 0 = 1) 
+            then nth_carry_sub_acc 1 n n a b  else nth_carry_sub_acc 0 n n a b)
+    else (if (nth_bit_tail a (n-diff+1) = 0 \<and> ( nth_bit_tail b (n-diff+1) = 1 \<or> acc = 1))
+                \<or> (nth_bit_tail a (n-diff+1) = 1 \<and> (nth_bit_tail b (n-diff+1) ) = 1 \<and> acc = 1)
+           then  nth_carry_sub_acc 1 (diff -1) n a b
+            else nth_carry_sub_acc 0 (diff - 1) n a b))
+)  "
+
+
+lemma nth_carry_sub_step:"diff < n \<Longrightarrow> nth_carry_sub_acc (nth_carry_sub_nat (n- Suc diff) a b ) (Suc diff) n a b 
+=  nth_carry_sub_acc (nth_carry_sub_nat (n-diff) a b) diff n a b "
+  apply (subst (1) nth_carry_sub_acc.simps )
+  apply (subst (1) nth_carry_sub_nat.simps)
+  apply (auto simp add: Suc_diff_Suc subtail_nth_bit 
+            simp del: nth_carry_sub_acc.simps nth_bit_nat.simps nth_carry_sub_nat.simps simp flip: One_nat_def)
+  apply (metis One_nat_def  nth_carry_sub_nat.elims)
+  apply auto
+  done
+lemma nth_carry_sub_induct:"diff \<le>n \<Longrightarrow> nth_carry_sub_acc (nth_carry_sub_nat (n-diff) a b) diff n a b
+= nth_carry_sub_nat n a b"
+  apply (induct diff)
+  apply simp
+   apply (auto simp add: nth_carry_sub_step simp del:nth_carry_sub_acc.simps nth_carry_sub_nat.simps )
+  done
+lemma nth_carry_sub_base:"nth_carry_sub_nat 0 a b = (if (nth_bit_nat a 0 = 0 \<and> nth_bit_nat b 0 = 1) 
+            then 1 else 0)" 
+  apply auto
   done
 
+definition nth_carry_sub_tail :: "nat \<Rightarrow> nat \<Rightarrow> nat \<Rightarrow> nat" where 
+"nth_carry_sub_tail n a b = nth_carry_sub_acc 0 (Suc n) n a b"
 
+lemma subtail_nth_carry_sub:
+"nth_carry_sub_tail n a b
+= nth_carry_sub_nat n a b"
+  apply (auto simp only: nth_carry_sub_tail_def)
+  apply (subst nth_carry_sub_acc.simps)
+  using nth_carry_sub_induct[of n n a b] nth_carry_sub_base subtail_nth_bit
+   apply (auto simp add:  simp del:nth_carry_sub_acc.simps nth_carry_sub_nat.simps nth_bit_nat.simps )
+  done
 
 fun bit_list_to_nat_nat:: "nat \<Rightarrow> nat" where
 "bit_list_to_nat_nat n = (if n =0 then 0 else if hd_nat n =0 then 2 *bit_list_to_nat_nat (tl_nat n)
@@ -69,6 +156,118 @@ lemma sub_bit_list_to_nat: "bit_list_to_nat_nat (list_encode (map bit_encode x))
           sub_head_map bit_list_to_nat.simps split:bit.splits)
    apply (auto)
   done
+fun bit_list_to_nat_acc:: "nat \<Rightarrow> nat \<Rightarrow> nat" where
+"bit_list_to_nat_acc acc n = (if n =0 then acc else if hd_nat n =0 then bit_list_to_nat_acc (2*acc) (tl_nat n)
+   else  bit_list_to_nat_acc (2*acc +1) (tl_nat n))"
 
 
+fun reverse_nat_acc :: "nat \<Rightarrow>nat \<Rightarrow> nat" where 
+"reverse_nat_acc acc n = (if n = 0 then acc else reverse_nat_acc ((hd_nat n) ## acc) (tl_nat n) )"
+
+lemma sub_reverse_nat_acc:"reverse_nat_acc (list_encode acc) (list_encode n) = list_encode (rev n @ acc) "
+  apply(induct n arbitrary: acc)
+  apply simp
+  apply(subst reverse_nat_acc.simps)
+  apply(auto simp only:sub_hd head.simps sub_tl tail.simps sub_cons rev.simps)
+  apply auto
+  done
+
+definition reverse_nat :: "nat \<Rightarrow> nat" where 
+"reverse_nat n = reverse_nat_acc 0 n"
+
+lemma sub_reverse:"reverse_nat (list_encode n) = list_encode (rev n)"
+  apply(auto simp only: reverse_nat_def )
+  using sub_reverse_nat_acc list_encode.simps(1) 
+  by (metis append_Nil2)
+lemma reverse_nat_0:"(reverse_nat 0 =0)" by (auto simp add:reverse_nat_def)
+
+lemma append_rev_nat:"append_nat (reverse_nat (Suc v)) xs = append_nat (reverse_nat (tl_nat (Suc v))) ((hd_nat (Suc v)) ## xs)"
+proof-
+  obtain ys where xs_def: "Suc v = list_encode ys" 
+    by (metis list_decode_inverse)
+  then moreover obtain a ys' where xs_def_cons : "ys = a#ys'"
+    by (metis list_encode.elims nat.simps(3))
+  moreover obtain xs_list where "xs = list_encode xs_list"  by (metis list_decode_inverse)
+  ultimately show ?thesis by (auto simp add: sub_reverse sub_tl sub_hd sub_cons 
+          sub_append simp del: list_encode.simps)
+qed
+lemma append_cons_nat_0 : "append_nat xs (a ## ys) \<noteq> 0"
+proof-
+  obtain ys' where xs_def: "ys = list_encode ys'" 
+    by (metis list_decode_inverse)
+  moreover obtain xs' where xs_def_cons : "xs = list_encode xs'"
+   by (metis list_decode_inverse)
+  ultimately show ?thesis by (auto simp add: sub_reverse sub_tl sub_hd sub_cons 
+          sub_append list_encode_eq simp flip: list_encode.simps)
+qed
+lemma cons_Nil:"xs ## ys \<noteq> 0"
+proof-
+  obtain ys' where xs_def: "ys = list_encode ys'" 
+    by (metis list_decode_inverse)
+  then show ?thesis by (auto simp add: sub_cons 
+          list_encode_eq simp flip: list_encode.simps)
+qed
+lemma tl_cons: "tl_nat (a##ys) = ys"
+proof-
+  obtain ys' where xs_def: "ys = list_encode ys'" 
+    by (metis list_decode_inverse)
+  then show ?thesis by (auto simp add: sub_cons sub_tl
+          list_encode_eq simp flip: list_encode.simps)
+qed
+
+lemma hd_cons: "hd_nat (a##ys) = a"
+proof-
+  obtain ys' where xs_def: "ys = list_encode ys'" 
+    by (metis list_decode_inverse)
+  then show ?thesis by (auto simp add: sub_cons sub_hd
+          list_encode_eq simp flip: list_encode.simps)
+qed
+lemma rev_rev_nat: "reverse_nat (reverse_nat ys) = ys"
+ proof-
+  obtain ys' where xs_def: "ys = list_encode ys'" 
+    by (metis list_decode_inverse)
+  then show ?thesis by (auto simp add: sub_cons sub_reverse sub_hd
+          list_encode_eq simp flip: list_encode.simps)
+qed
+lemma bit_list_to_nat_induct: "bit_list_to_nat_nat (append_nat (reverse_nat ys) xs) = bit_list_to_nat_acc (bit_list_to_nat_nat xs) ys"
+  apply(induct ys arbitrary:xs rule: length_nat.induct)
+  apply (auto simp only: reverse_nat_0 append_nat.simps)
+  apply(subst bit_list_to_nat_acc.simps)
+   apply(auto simp del: bit_list_to_nat_nat.simps bit_list_to_nat_acc.simps 
+          simp add: append_rev_nat )
+  apply(subst(2) bit_list_to_nat_acc.simps)
+     apply(auto simp del: bit_list_to_nat_nat.simps bit_list_to_nat_acc.simps cons_def
+          simp add: append_rev_nat )
+     apply(subst bit_list_to_nat_nat.simps)
+          apply(auto simp del:   bit_list_to_nat_nat.simps bit_list_to_nat_acc.simps cons_def
+          simp add: append_cons_nat_0 cons_Nil tl_cons hd_cons)
+  apply(subst bit_list_to_nat_nat.simps)
+ apply(auto simp del:   bit_list_to_nat_nat.simps bit_list_to_nat_acc.simps cons_def
+          simp add: append_cons_nat_0 cons_Nil tl_cons hd_cons)
+  done
+
+lemma append_nat_0: "append_nat ys 0 = ys"
+proof-
+  obtain ys' where xs_def: "ys = list_encode ys'" 
+    by (metis list_decode_inverse)
+  then show ?thesis by (auto simp add: sub_append sub_hd
+          list_encode_eq simp flip: list_encode.simps)
+qed
+
+lemma bit_list_to_nat_inverse: 
+"bit_list_to_nat_nat (append_nat ys xs) = bit_list_to_nat_acc (bit_list_to_nat_nat xs) (reverse_nat ys)"
+  using rev_rev_nat bit_list_to_nat_induct by metis
+
+definition bit_list_to_nat_tail :: "nat \<Rightarrow> nat" where 
+"bit_list_to_nat_tail ys =  bit_list_to_nat_acc 0 (reverse_nat ys)"
+
+lemma subtail_bit_list_to_nat:
+" bit_list_to_nat_tail ys = bit_list_to_nat_nat ys"
+  using bit_list_to_nat_inverse [of ys 0] append_nat_0 
+  by (auto simp add: bit_list_to_nat_tail_def)
+
+
+
+
+  
 end
