Cook_Levin/IMP-_To_SAS+/IMP-_To_IMP--/Primitives.thy
@@ -965,6 +965,16 @@ fun map_list_find_nat :: "nat \<Rightarrow> nat \<Rightarrow> nat" where
 "map_list_find_nat xs a = (if xs = 0 then 0 else if fst_nat (hd_nat xs) = a then some_nat (snd_nat (hd_nat xs))  
   else map_list_find_nat (tl_nat xs) a) "
 
+fun map_list_find_tail :: "nat \<Rightarrow> nat \<Rightarrow> nat" where 
+"map_list_find_tail xs a = (if xs = 0 then 0 else if fst_nat (hd_nat xs) = a then some_nat (snd_nat (hd_nat xs))  
+  else map_list_find_nat (tl_nat xs) a) "
+
+lemma subtail_map_list_find:
+"map_list_find_tail xs a = map_list_find_nat xs a"
+  apply(induct xs a rule: map_list_find_nat.induct)
+  apply auto
+  done
+
 lemma sub_map_list_find_nat:
       "map_list_find_nat (list_encode (map prod_encode xs)) a =
         option_encode (map_list_find xs a)"
@@ -1031,6 +1041,13 @@ lemma sub_fun_list_find:"fun_list_find xs a = fun_of xs a"
 fun fun_list_find_nat :: "nat \<Rightarrow> nat \<Rightarrow> nat" where 
 "fun_list_find_nat xs a  = (if xs = 0 then 0 else if fst_nat (hd_nat xs) = a then snd_nat (hd_nat xs) else fun_list_find_nat (tl_nat xs) a) "
 
+fun fun_list_find_tail :: "nat \<Rightarrow> nat \<Rightarrow> nat" where 
+"fun_list_find_tail xs a  = (if xs = 0 then 0 else if fst_nat (hd_nat xs) = a then snd_nat (hd_nat xs) else fun_list_find_tail (tl_nat xs) a) "
+
+lemma subtail_fun_list_find: "fun_list_find_tail xs a = fun_list_find_nat xs a"
+  apply(induct xs a rule: fun_list_find_tail.induct)
+  apply auto
+  done
 
 lemma sub_fun_list_find_nat :
  "fun_list_find_nat (list_encode (map prod_encode xs)) a = fun_list_find xs a"
